Minor cleanup 011-string_xor

011-string_xor.dfy
@@ -1,27 +1,28 @@
-method xor(a : char, b : char) returns (result : char)
-    // post-conditions-start
-    ensures result == (if a == b then '0' else '1')
-    // post-conditions-end
+predicate represents_byte(a: char)
 {
-    // impl-start
-    if (a == b) {
-        result := '0';
-    } else {
-        result := '1';
-    }
-    // impl-end
+    a in "01"
+}
+
+function char_xor(a: char, b: char): char
+    requires represents_byte(a)
+    requires represents_byte(b)
+{
+    if (a == b) then
+        '0'
+    else
+        '1'
 }
 
 method string_xor(a: string, b: string) returns (result: string)
     // pre-conditions-start
     requires |a| == |b|
-    requires forall i :: 0 <= i < |a| ==> (a[i] == '0' || a[i] == '1')
-    requires forall i :: 0 <= i < |b| ==> (b[i] == '0' || b[i] == '1')
+    requires forall i :: 0 <= i < |a| ==> represents_byte(a[i])
+    requires forall i :: 0 <= i < |b| ==> represents_byte(b[i])
     // pre-conditions-end
     // post-conditions-start
     ensures |result| == |a|
-    ensures forall i :: 0 <= i < |result| ==> (result[i] == '0' || result[i] == '1')
-    ensures forall i :: 0 <= i < |result| ==> result[i] == (if a[i] == b[i] then '0' else '1')
+    ensures forall i :: 0 <= i < |result| ==> represents_byte(result[i])
+    ensures forall i :: 0 <= i < |result| ==> result[i] == char_xor(a[i], b[i])
     // post-conditions-end
 {
     // impl-start
@@ -29,12 +30,14 @@ method string_xor(a: string, b: string) returns (result: string)
     var i : int := 0;
     while (i < |a|)
         // invariants-start
-        invariant i >= 0 && i <= |a|
+        invariant 0 <= i <= |a|
         invariant |result| == i
-        invariant forall j :: 0 <= j < i ==> result[j] == (if a[j] == b[j] then '0' else '1')
+        invariant forall i :: 0 <= i < |a| ==> represents_byte(a[i])
+        invariant forall i :: 0 <= i < |b| ==> represents_byte(b[i])
+        invariant forall j :: 0 <= j < i ==> result[j] == char_xor(a[j], b[j])
         // invariants-end
     {
-        var bitResult := if a[i] == b[i] then '0' else '1';
+        var bitResult := char_xor(a[i], b[i]);
         result := result + [bitResult];
         i := i + 1;
     }
